\documentclass{ximera}
\input{../preamble}
\addPrintStyle{..}
\begin{document}
	\author{Wiskunde Op Maat}
	\xmtitle{Lineaire vergelijkingen oplossen}{}

\begin{exercise} Los volgende lineaire vergelijking op naar de onbekende \(x\).
\begin{xmmulticols}
  
  \begin{question} \( 3x + 7  =  2x + 12    \) \begin{oplossing} \( x  = 5  \) \end{oplossing} \end{question}
  \begin{question} \( 4x - 5  =  3x + 8     \) \begin{oplossing} \( x  = 13 \) \end{oplossing} \end{question}
  \begin{question} \( 6x + 2  =  5x + 10    \) \begin{oplossing} \( x  = 8  \) \end{oplossing} \end{question}
  \begin{question} \( 7x - 3  =  4x + 9     \) \begin{oplossing} \( x  = 4  \) \end{oplossing} \end{question}
  \begin{question} \( 5x + 1  =  3x + 7     \) \begin{oplossing} \( x  = 3  \) \end{oplossing} \end{question}
  \begin{question} \( 2x + 9  =  4x - 5     \) \begin{oplossing} \( x  = 7  \) \end{oplossing} \end{question}
  \begin{question} \( 9x - 6  =  3x + 12    \) \begin{oplossing} \( x  = 3  \) \end{oplossing} \end{question}
  \begin{question} \( 11x + 4 =  5x + 22    \) \begin{oplossing} \( x  = 3  \) \end{oplossing} \end{question}
  \begin{question} \( 6x + 3  =  2x + 15    \) \begin{oplossing} \( x  = 3  \) \end{oplossing} \end{question}
  \begin{question} \( 4x - 9  =  3x + 1     \) \begin{oplossing} \( x  = 10 \) \end{oplossing} \end{question}
  \begin{question} \( 8x + 5  =  2x + 29    \) \begin{oplossing} \( x  = 4  \) \end{oplossing} \end{question}
  \begin{question} \( 7x - 2  =  5x + 8     \) \begin{oplossing} \( x  = 5  \) \end{oplossing} \end{question}
  \begin{question} \( 10x + 6 =  4x + 30    \) \begin{oplossing} \( x  = 4  \) \end{oplossing} \end{question}
  \begin{question} \( 12x - 7 =  6x + 11    \) \begin{oplossing} \( x  = 3  \) \end{oplossing} \end{question}
  \begin{question} \( 5x + 2  =  3x + 10    \) \begin{oplossing} \( x  = 4  \) \end{oplossing} \end{question}
  \begin{question} \( 6x - 1  =  4x + 9     \) \begin{oplossing} \( x  = 5  \) \end{oplossing} \end{question}
  \begin{question} \( 9x - 8  =  4x + 7     \) \begin{oplossing} \( x  = 3  \) \end{oplossing} \end{question}
  \begin{question} \( 3x + 5  =  2x + 11    \) \begin{oplossing} \( x  = 6  \) \end{oplossing} \end{question}
  \begin{question} \( 4x + 2  =  10         \) \begin{oplossing} \( x  = 2  \) \end{oplossing} \end{question}
  \begin{question} \( 7x + 1  =  4x + 10    \) \begin{oplossing} \( x  = 3  \) \end{oplossing} \end{question}
  \begin{question} \( 5x + 9  =  2x + 18    \) \begin{oplossing} \( x  = 3  \) \end{oplossing} \end{question}
  \begin{question} \( 3x - 4  =  x + 6      \) \begin{oplossing} \( x  = 5  \) \end{oplossing} \end{question}
  \begin{question} \( 2x + 7  =  13         \) \begin{oplossing} \( x  = 3  \) \end{oplossing} \end{question}
  \begin{question} \( 6x - 4  =  2x + 12    \) \begin{oplossing} \( x  = 4  \) \end{oplossing} \end{question}
  \begin{question} \( 4x + 8  =  24         \) \begin{oplossing} \( x  = 4  \) \end{oplossing} \end{question}
  \begin{question} \( 11x + 8 =  5x + 26    \) \begin{oplossing} \( x  = 3  \) \end{oplossing} \end{question}
  \begin{question} \( 3x - 4  =  8          \) \begin{oplossing} \( x  = 4  \) \end{oplossing} \end{question}
  \begin{question} \( 5x + 6  =  26         \) \begin{oplossing} \( x  = 4  \) \end{oplossing} \end{question}
  \begin{question} \( 7x - 3  =  2x + 12    \) \begin{oplossing} \( x  = 3  \) \end{oplossing} \end{question}
  \begin{question} \( 9x + 5  =  50         \) \begin{oplossing} \( x  = 5  \) \end{oplossing} \end{question}
  
\end{xmmulticols}
\end{exercise}

\begin{exercise} Los volgende lineaire vergelijking op naar de onbekende \(x\).
\begin{xmmulticols}
  
  
  \begin{question} \( 4x - 7  =  3x + 1     \) \begin{oplossing} \( x  = 8  \) \end{oplossing} \end{question}
  \begin{question} \( 8x - 4  =  28         \) \begin{oplossing} \( x  = 4  \) \end{oplossing} \end{question}
  \begin{question} \( 11x + 9 =  5x + 21    \) \begin{oplossing} \( x  = 2  \) \end{oplossing} \end{question}
  \begin{question} \( x + 7   =  12         \) \begin{oplossing} \( x  = 5  \) \end{oplossing} \end{question}
  \begin{question} \( 3x - 5  =  x + 7      \) \begin{oplossing} \( x  = 6  \) \end{oplossing} \end{question}
  \begin{question} \( x - 9   =  -2         \) \begin{oplossing} \( x  = 7  \) \end{oplossing} \end{question}
  \begin{question} \( 2x + 5  =  11         \) \begin{oplossing} \( x  = 3  \) \end{oplossing} \end{question}
  \begin{question} \( 7x + 2  =  3x + 10    \) \begin{oplossing} \( x  = 2  \) \end{oplossing} \end{question}
  \begin{question} \( 7x + 4  =  25         \) \begin{oplossing} \( x  = 3  \) \end{oplossing} \end{question}
  \begin{question} \( 2x + 6  =  5x - 9     \) \begin{oplossing} \( x  = 5  \) \end{oplossing} \end{question}
  \begin{question} \( 4x - 5  =  11         \) \begin{oplossing} \( x  = 4  \) \end{oplossing} \end{question}
  \begin{question} \( 6x - 2  =  3x + 10    \) \begin{oplossing} \( x  = 4  \) \end{oplossing} \end{question}
  \begin{question} \( 6x - 7  =  11         \) \begin{oplossing} \( x  = 3  \) \end{oplossing} \end{question}
  \begin{question} \( 3x - 5  =  10         \) \begin{oplossing} \( x  = 5  \) \end{oplossing} \end{question}
  \begin{question} \( 10x - 3 =  4x + 15    \) \begin{oplossing} \( x  = 3  \) \end{oplossing} \end{question}
  \begin{question} \( 7x + 4  =  2x + 19    \) \begin{oplossing} \( x  = 3  \) \end{oplossing} \end{question}
  \begin{question} \( 5x - 6  =  2x + 9     \) \begin{oplossing} \( x  = 5  \) \end{oplossing} \end{question}
  \begin{question} \( 3x + 7  =  x + 15     \) \begin{oplossing} \( x  = 4  \) \end{oplossing} \end{question}
  \begin{question} \( 10x + 2 =  32         \) \begin{oplossing} \( x  = 3  \) \end{oplossing} \end{question}
  \begin{question} \( x - 6   =  -1         \) \begin{oplossing} \( x  = 5  \) \end{oplossing} \end{question}

\end{xmmulticols}
\end{exercise}


\end{document}


